code/rocq/wip/lang.v
@@ -305,31 +305,37 @@ Module Run (U : Unif).
       by left; apply: dead_failed H1.
   Qed.
 
+  Definition is_base X := match X with Top | Bot | Goal _ _ => true | _ => false end.
 
-  Fixpoint next_alt_aux inAnd (s : Sigma) (A : state) : option (Sigma * state) :=
+
+  Fixpoint next_alt_aux (s : Sigma) (A : state) : option (Sigma * state) :=
     match A with
     | KO | OK => None
     | Dead => None
-    | Top | Bot | Goal _ _ => if inAnd then None else Some (s, A)
+    | Top | Bot | Goal _ _ => None
     | And A B0 B =>
-      match next_alt_aux true s B, next_alt_aux true s A with
+      match next_alt_aux s B, next_alt_aux s A with
       | None, None => None
       | None, Some (s, A) => Some (s, And A B0 B0) (* B0 è un grande and di ATOMI *)
       | Some (s, B), _ => Some (s, And A B0 B)
       end
     | Or A sB B => 
       if A == dead A then
-        match next_alt_aux false s B with
+        if is_base B then Some (s, Or A sB B) 
+        else
+        match next_alt_aux s B with
         | None => None
         | Some (sB1, B) => if B == dead B then None else Some (sB1, Or A sB B)
         end
       else
         if B == dead B then None else
-        match next_alt_aux false s A with
+        match next_alt_aux s A with
         | None =>  Some (sB, Or (dead A) sB B)
         | Some (sA, A) => Some (sA, Or A sB B)
         end
     end.
+
+  Definition has_next_alt_aux s := isSome (next_alt_aux empty s).
 
   Lemma cut_dead1 {A}: cut A = dead A -> dead A = A.
   Proof. 
@@ -338,9 +344,9 @@ Module Run (U : Unif).
     move=> A HA B0 _ B HB/=[]??; rewrite HA//HB//.
   Qed.
   Inductive next_alt : Sigma -> state -> option (Sigma * state) -> Prop :=
-    | next_alt_ko {s A}: next_alt_aux false s A = None -> next_alt s A None
-    | next_alt_ok {s s1 A A1}: next_alt_aux false s A = Some (s1, A1) -> ~ failed A1 -> next_alt s A (Some (s1, A1))
-    | next_alt_step {s s1 r A A1}: next_alt_aux false s A = Some (s1, A1) -> failed A1 -> next_alt s1 A1 r -> next_alt s A r.
+    | next_alt_ko {s A}: next_alt_aux s A = None -> next_alt s A None
+    | next_alt_ok {s s1 A A1}: next_alt_aux s A = Some (s1, A1) -> ~ failed A1 -> next_alt s A (Some (s1, A1))
+    | next_alt_step {s s1 r A A1}: next_alt_aux s A = Some (s1, A1) -> failed A1 -> next_alt s1 A1 r -> next_alt s A r.
 
   Inductive run_res := Done of Sigma & state | Failed of state.
   derive run_res.
@@ -544,7 +550,6 @@ Module Run (U : Unif).
   Qed.
 
   Definition is_meta X := match X with OK | KO | Dead => true | _ => false end.
-  Definition is_base X := match X with Top | Bot | Goal _ _ => true | _ => false end.
 
   (* Lemma simpl_next_alt_aux_false {s1 s2 A B r}: 
     next_alt_aux false s1 (Or A s2 B) = Some r -> 
@@ -559,20 +564,30 @@ Module Run (U : Unif).
     + move=> /=; case Y: next_alt_aux => [[ ]|].
       + move=> [] ?.  *)
 
-  Lemma next_alt_aux_dead {b s1 s3 A B}: 
-    next_alt_aux b s1 A = Some (s3, B) -> B <> dead B.
+  Lemma simpl_is_base {B}: is_base B -> B = Top \/ B = Bot \/ (exists p t, B = Goal p t).
+  Proof. by case B => //=; auto; right; right; do 2 eexists. Qed.
+
+  Lemma next_alt_aux_dead {s1 s3 A B}: 
+    next_alt_aux s1 A = Some (s3, B) -> B <> dead B.
   Proof.
-    elim: A b B s1 s3; try by move=>/=[]//[]//.
-    + by move=>??/=[]//[]//.
-    + move=> A HA s B HB b/=C s1 s2.
+    elim: A B s1 s3; try by move=>/=[]//[]//.
+    (* + by move=>??/=[]//[]//. *)
+    + move=> A HA s B HB/=C s1 s2.
       case: ifP => [/eqP->|/eqP].
+        case: ifP => //.
+          move=>/simpl_is_base[].
+            move=>->-[]*; subst => //.
+          move=>[].
+            move=>->-[]*; subst => //.
+          move=>[?[?]]->[]*;subst => //.
+        move=> _.
         case NA: next_alt_aux => //[[s3 D]].
         case: ifP => ///eqP DD []?? /=; subst => -[].
         rewrite dead_dead_same; congruence.
       move=> DA.
       case: ifP => ///eqP H.
       case NA: next_alt_aux => [[s3 D]|] => -[]*; subst => -[]//.
-    + move=> A HA B0 _ B HB s1 C s2 s3/=.
+    + move=> A HA B0 _ B HB s1 s2 s3/=.
       case NB: next_alt_aux => // [[s4 D]|].
         move=>[]*;subst => /= => -[]*; subst.
         by apply: HB NB _.
@@ -587,50 +602,50 @@ Module Run (U : Unif).
     | _, _ => false
     end.
 
-  Lemma next_alt_aux_same_sol s1 s2 A b:
-    same_sol (next_alt_aux b s1 A) (next_alt_aux b s2 A).
+  Lemma next_alt_aux_same_sol s1 s2 A:
+    same_sol (next_alt_aux s1 A) (next_alt_aux s2 A).
   Proof.
-    elim: A b s1 s2 => //; try by move=> [] *; subst.
-    + by move=> ??[]/=.
-    + move=> A HA s B HB b s1 s2 /=.
+    elim: A s1 s2 => //; try by move=> [] *; subst.
+    (* + by move=> ??[]/=. *)
+    + move=> A HA s B HB s1 s2 /=.
       case:ifP => /eqP.
         move=>->.
-        case NB: next_alt_aux => [[s5 E]|]; have:= HB false s1 s2; rewrite /= NB/=.
-          case: next_alt_aux => // [[s4 D]]/eqP->/=.
-          case: ifP => //=.
-        case:next_alt_aux => //.
+        case: ifP.  
+          by move=>/simpl_is_base[->|[->|[?[?->]]]]/=.
+        move=> H.
+        have:= HB s1 s2.
+        case: next_alt_aux => //[[s5 E]|]; case: next_alt_aux => //[[s6 F]].
+        move=> /=/eqP->; case: ifP => //=.
       case: ifP => /eqP//DB DA.
-      case NA: next_alt_aux => [[s3 C]|]; have:= HA false s1 s2; rewrite NA.
+      have:= HA s1 s2.
+      case NA: next_alt_aux => [[s3 C]|].
         by case: next_alt_aux => // [[s4 D]]/eqP->/=; rewrite eqxx.
       case: next_alt_aux => //=.
-    + move=> A HA B0 _ B HB b s1 s2 /=.
+    + move=> A HA B0 _ B HB s1 s2 /=.
+      have:= HB s1 s2.
       case NB: next_alt_aux => [[s3 C]|].
-        have:= HB true s1 s2; rewrite NB.
         by case: next_alt_aux => [[s4 D]|]///eqP->/=.
-      have:= HB true s1 s2; rewrite NB.
-        case: (next_alt_aux true s2 B) => // _.
-      case NA: next_alt_aux => [[s3 C]|].
-        have:= HA true s1 s2; rewrite NA.
-        by case: next_alt_aux => //[[s4 D]]/eqP-> //=.
-      have:= HA true s1 s2; rewrite NA.
-      by case: next_alt_aux => //=.
+      case: next_alt_aux => // _.
+      have:= HA s1 s2.
+      case: next_alt_aux => //=[[s3 C]|]; case: next_alt_aux => //[[s4 D]].
+      by move=>/eqP ->/=.
   Qed.
 
-  Lemma next_alt_aux_none {s1 A b}:
-    next_alt_aux b s1 A = None ->
-      forall s2, next_alt_aux b s2 A = None.
+  Lemma next_alt_aux_none {s1 A}:
+    next_alt_aux s1 A = None ->
+      forall s2, next_alt_aux s2 A = None.
   Proof.
     move=> H s2.
-    have := next_alt_aux_same_sol s1 s2 A b.
+    have := next_alt_aux_same_sol s1 s2 A.
     rewrite H => /=; case: next_alt_aux => //.
   Qed.
 
-  Lemma next_alt_aux_some {s1 s2 A B b}:
-    next_alt_aux b s1 A = Some (s2, B) ->
-      (forall s3, exists s4, next_alt_aux b s3 A = Some (s4, B)).
+  Lemma next_alt_aux_some {s1 s2 A B}:
+    next_alt_aux s1 A = Some (s2, B) ->
+      (forall s3, exists s4, next_alt_aux s3 A = Some (s4, B)).
   Proof.
     move=> H s3.
-    have := next_alt_aux_same_sol s1 s3 A b.
+    have := next_alt_aux_same_sol s1 s3 A.
     rewrite H/=.
     by case X: next_alt_aux => // [[s4 C]]/eqP->; eexists.
   Qed.
@@ -648,7 +663,7 @@ Module Run (U : Unif).
   Qed.
 
   Lemma simpl_next_alt_aux_and_none {s A B0 B}:
-    next_alt_aux true s (And A B0 B) = None -> next_alt_aux true s B = None /\  next_alt_aux true s A = None.
+    next_alt_aux s (And A B0 B) = None -> next_alt_aux s B = None /\  next_alt_aux s A = None.
   Proof. 
     rewrite /next_alt //=. 
     case X: next_alt_aux => [x|].
@@ -656,7 +671,7 @@ Module Run (U : Unif).
     + by case Y: next_alt_aux => [x|] //; case x.
   Qed.
 
-  Lemma simpl_next_alt_aux_some {b s s1 s2 A B C}: next_alt_aux b s1 (Or A s B) = Some (s2, C) -> 
+  (* Lemma simpl_next_alt_aux_some {b s s1 s2 A B C}: next_alt_aux b s1 (Or A s B) = Some (s2, C) -> 
     (exists B', A = dead A /\ next_alt_aux false s1 B = Some (s2, B') /\ C = Or A s B') \/
     (A <> dead A /\ B <> dead B /\ 
       ((exists A', next_alt_aux false s1 A = Some (s2, A') /\ C = Or A' s B) \/
@@ -674,7 +689,7 @@ Module Run (U : Unif).
       left; eexists => //.
     right; repeat split => //.
     by right.
-  Qed.
+  Qed. *)
 
   Lemma success_dead {A}: success (dead A) = false.
   Proof. 
